tuned proofs; tuned white space; more symbols;

src/HOL/Library/DAList.thy
@@ -1,96 +1,107 @@
 (*  Title:      HOL/Library/DAList.thy
-    Author:     Lukas Bulwahn, TU Muenchen *)
+    Author:     Lukas Bulwahn, TU Muenchen
+*)
 
-header {* Abstract type of association lists with unique keys *}
+header \<open>Abstract type of association lists with unique keys\<close>
 
 theory DAList
 imports AList
 begin
 
-text {* This was based on some existing fragments in the AFP-Collection framework. *}
+text \<open>This was based on some existing fragments in the AFP-Collection framework.\<close>
 
-subsection {* Preliminaries *}
+subsection \<open>Preliminaries\<close>
 
 lemma distinct_map_fst_filter:
-   "distinct (map fst xs) ==> distinct (map fst (List.filter P xs))"
-by (induct xs) auto
+  "distinct (map fst xs) \<Longrightarrow> distinct (map fst (List.filter P xs))"
+  by (induct xs) auto
 
-subsection {* Type @{text "('key, 'value) alist" } *}
 
-typedef ('key, 'value) alist = "{xs :: ('key \<times> 'value) list. (distinct o map fst) xs}"
+subsection \<open>Type @{text "('key, 'value) alist" }\<close>
+
+typedef ('key, 'value) alist = "{xs :: ('key \<times> 'value) list. (distinct \<circ> map fst) xs}"
   morphisms impl_of Alist
 proof
-  show "[] \<in> {xs. (distinct o map fst) xs}" by simp
+  show "[] \<in> {xs. (distinct o map fst) xs}"
+    by simp
 qed
 
 setup_lifting type_definition_alist
 
 lemma alist_ext: "impl_of xs = impl_of ys \<Longrightarrow> xs = ys"
-by(simp add: impl_of_inject)
+  by (simp add: impl_of_inject)
 
 lemma alist_eq_iff: "xs = ys \<longleftrightarrow> impl_of xs = impl_of ys"
-by(simp add: impl_of_inject)
+  by (simp add: impl_of_inject)
 
 lemma impl_of_distinct [simp, intro]: "distinct (map fst (impl_of xs))"
-using impl_of[of xs] by simp
+  using impl_of[of xs] by simp
 
 lemma Alist_impl_of [code abstype]: "Alist (impl_of xs) = xs"
-by(rule impl_of_inverse)
+  by (rule impl_of_inverse)
 
-subsection {* Primitive operations *}
+
+subsection \<open>Primitive operations\<close>
 
 lift_definition lookup :: "('key, 'value) alist \<Rightarrow> 'key \<Rightarrow> 'value option" is map_of  .
 
-lift_definition empty :: "('key, 'value) alist" is "[]" by simp
+lift_definition empty :: "('key, 'value) alist" is "[]"
+  by simp
 
 lift_definition update :: "'key \<Rightarrow> 'value \<Rightarrow> ('key, 'value) alist \<Rightarrow> ('key, 'value) alist"
   is AList.update
-by (simp add: distinct_update)
+  by (simp add: distinct_update)
 
 (* FIXME: we use an unoptimised delete operation. *)
 lift_definition delete :: "'key \<Rightarrow> ('key, 'value) alist \<Rightarrow> ('key, 'value) alist"
   is AList.delete
-by (simp add: distinct_delete)
+  by (simp add: distinct_delete)
 
-lift_definition map_entry :: "'key \<Rightarrow> ('value \<Rightarrow> 'value) \<Rightarrow> ('key, 'value) alist \<Rightarrow> ('key, 'value) alist"
+lift_definition map_entry ::
+    "'key \<Rightarrow> ('value \<Rightarrow> 'value) \<Rightarrow> ('key, 'value) alist \<Rightarrow> ('key, 'value) alist"
   is AList.map_entry
-by (simp add: distinct_map_entry)
+  by (simp add: distinct_map_entry)
 
 lift_definition filter :: "('key \<times> 'value \<Rightarrow> bool) \<Rightarrow> ('key, 'value) alist \<Rightarrow> ('key, 'value) alist"
   is List.filter
-by (simp add: distinct_map_fst_filter)
+  by (simp add: distinct_map_fst_filter)
 
-lift_definition map_default :: "'key => 'value => ('value => 'value) => ('key, 'value) alist => ('key, 'value) alist"
+lift_definition map_default ::
+    "'key \<Rightarrow> 'value \<Rightarrow> ('value \<Rightarrow> 'value) \<Rightarrow> ('key, 'value) alist \<Rightarrow> ('key, 'value) alist"
   is AList.map_default
-by (simp add: distinct_map_default)
+  by (simp add: distinct_map_default)
 
-subsection {* Abstract operation properties *}
+
+subsection \<open>Abstract operation properties\<close>
 
 (* FIXME: to be completed *)
 
 lemma lookup_empty [simp]: "lookup empty k = None"
-by(simp add: empty_def lookup_def Alist_inverse)
+  by (simp add: empty_def lookup_def Alist_inverse)
 
 lemma lookup_delete [simp]: "lookup (delete k al) = (lookup al)(k := None)"
-by (simp add: lookup_def delete_def Alist_inverse distinct_delete delete_conv')
+  by (simp add: lookup_def delete_def Alist_inverse distinct_delete delete_conv')
 
-subsection {* Further operations *}
 
-subsubsection {* Equality *}
+subsection \<open>Further operations\<close>
 
-instantiation alist :: (equal, equal) equal begin
+subsubsection \<open>Equality\<close>
+
+instantiation alist :: (equal, equal) equal
+begin
 
 definition "HOL.equal (xs :: ('a, 'b) alist) ys == impl_of xs = impl_of ys"
 
 instance
-proof
-qed (simp add: equal_alist_def impl_of_inject)
+  by default (simp add: equal_alist_def impl_of_inject)
 
 end
 
-subsubsection {* Size *}
 
-instantiation alist :: (type, type) size begin
+subsubsection \<open>Size\<close>
+
+instantiation alist :: (type, type) size
+begin
 
 definition "size (al :: ('a, 'b) alist) = length (impl_of al)"
 
@@ -98,15 +109,15 @@ instance ..
 
 end
 
-subsection {* Quickcheck generators *}
+
+subsection \<open>Quickcheck generators\<close>
 
 notation fcomp (infixl "\<circ>>" 60)
 notation scomp (infixl "\<circ>\<rightarrow>" 60)
 
 definition (in term_syntax)
   valterm_empty :: "('key :: typerep, 'value :: typerep) alist \<times> (unit \<Rightarrow> Code_Evaluation.term)"
-where
-  "valterm_empty = Code_Evaluation.valtermify empty"
+  where "valterm_empty = Code_Evaluation.valtermify empty"
 
 definition (in term_syntax)
   valterm_update :: "'key :: typerep \<times> (unit \<Rightarrow> Code_Evaluation.term) \<Rightarrow>
@@ -115,9 +126,15 @@ definition (in term_syntax)
   ('key, 'value) alist \<times> (unit \<Rightarrow> Code_Evaluation.term)" where
   [code_unfold]: "valterm_update k v a = Code_Evaluation.valtermify update {\<cdot>} k {\<cdot>} v {\<cdot>}a"
 
-fun (in term_syntax) random_aux_alist 
+fun (in term_syntax) random_aux_alist
 where
-  "random_aux_alist i j = (if i = 0 then Pair valterm_empty else Quickcheck_Random.collapse (Random.select_weight [(i, Quickcheck_Random.random j \<circ>\<rightarrow> (%k. Quickcheck_Random.random j \<circ>\<rightarrow> (%v. random_aux_alist (i - 1) j \<circ>\<rightarrow> (%a. Pair (valterm_update k v a))))), (1, Pair valterm_empty)]))"
+  "random_aux_alist i j =
+    (if i = 0 then Pair valterm_empty
+     else Quickcheck_Random.collapse
+       (Random.select_weight
+         [(i, Quickcheck_Random.random j \<circ>\<rightarrow> (\<lambda>k. Quickcheck_Random.random j \<circ>\<rightarrow>
+           (\<lambda>v. random_aux_alist (i - 1) j \<circ>\<rightarrow> (\<lambda>a. Pair (valterm_update k v a))))),
+          (1, Pair valterm_empty)]))"
 
 instantiation alist :: (random, random) random
 begin
@@ -125,7 +142,7 @@ begin
 definition random_alist
 where
   "random_alist i = random_aux_alist i i"
- 
+
 instance ..
 
 end
@@ -136,10 +153,19 @@ no_notation scomp (infixl "\<circ>\<rightarrow>" 60)
 instantiation alist :: (exhaustive, exhaustive) exhaustive
 begin
 
-fun exhaustive_alist :: "(('a, 'b) alist => (bool * term list) option) => natural => (bool * term list) option"
+fun exhaustive_alist ::
+  "(('a, 'b) alist \<Rightarrow> (bool \<times> term list) option) \<Rightarrow> natural \<Rightarrow> (bool \<times> term list) option"
 where
-  "exhaustive_alist f i = (if i = 0 then None else case f empty of Some ts => Some ts | None =>
-     exhaustive_alist (%a. Quickcheck_Exhaustive.exhaustive (%k. Quickcheck_Exhaustive.exhaustive (%v. f (update k v a)) (i - 1)) (i - 1)) (i - 1))"
+  "exhaustive_alist f i =
+    (if i = 0 then None
+     else
+      case f empty of
+        Some ts \<Rightarrow> Some ts
+      | None \<Rightarrow>
+          exhaustive_alist
+            (\<lambda>a. Quickcheck_Exhaustive.exhaustive
+              (\<lambda>k. Quickcheck_Exhaustive.exhaustive (\<lambda>v. f (update k v a)) (i - 1)) (i - 1))
+            (i - 1))"
 
 instance ..
 
@@ -148,10 +174,22 @@ end
 instantiation alist :: (full_exhaustive, full_exhaustive) full_exhaustive
 begin
 
-fun full_exhaustive_alist :: "(('a, 'b) alist * (unit => term) => (bool * term list) option) => natural => (bool * term list) option"
+fun full_exhaustive_alist ::
+  "(('a, 'b) alist \<times> (unit \<Rightarrow> term) \<Rightarrow> (bool \<times> term list) option) \<Rightarrow> natural \<Rightarrow>
+    (bool \<times> term list) option"
 where
-  "full_exhaustive_alist f i = (if i = 0 then None else case f valterm_empty of Some ts => Some ts | None =>
-     full_exhaustive_alist (%a. Quickcheck_Exhaustive.full_exhaustive (%k. Quickcheck_Exhaustive.full_exhaustive (%v. f (valterm_update k v a)) (i - 1)) (i - 1)) (i - 1))"
+  "full_exhaustive_alist f i =
+    (if i = 0 then None
+     else
+      case f valterm_empty of
+        Some ts \<Rightarrow> Some ts
+      | None \<Rightarrow>
+          full_exhaustive_alist
+            (\<lambda>a.
+              Quickcheck_Exhaustive.full_exhaustive
+                (\<lambda>k. Quickcheck_Exhaustive.full_exhaustive (\<lambda>v. f (valterm_update k v a)) (i - 1))
+              (i - 1))
+            (i - 1))"
 
 instance ..
 
@@ -160,6 +198,6 @@ end
 hide_const valterm_empty valterm_update random_aux_alist
 
 hide_fact (open) lookup_def empty_def update_def delete_def map_entry_def filter_def map_default_def
-hide_const (open) impl_of lookup empty update delete map_entry filter map_default 
+hide_const (open) impl_of lookup empty update delete map_entry filter map_default
 
 end
