src/HOL/Library/DAList_Multiset.thy
@@ -2,166 +2,144 @@
     Author:     Lukas Bulwahn, TU Muenchen
 *)
 
-header {* Multisets partially implemented by association lists *}
+header \<open>Multisets partially implemented by association lists\<close>
 
 theory DAList_Multiset
 imports Multiset DAList
 begin
 
-text {* Delete prexisting code equations *}
+text \<open>Delete prexisting code equations\<close>
 
-lemma [code, code del]:
-  "{#} = {#}"
-  ..
+lemma [code, code del]: "{#} = {#}" ..
 
-lemma [code, code del]:
-  "single = single"
-  ..
+lemma [code, code del]: "single = single" ..
 
-lemma [code, code del]:
-  "plus = (plus :: 'a multiset \<Rightarrow> _)"
-  ..
+lemma [code, code del]: "plus = (plus :: 'a multiset \<Rightarrow> _)" ..
 
-lemma [code, code del]:
-  "minus = (minus :: 'a multiset \<Rightarrow> _)"
-  ..
+lemma [code, code del]: "minus = (minus :: 'a multiset \<Rightarrow> _)" ..
 
-lemma [code, code del]:
-  "inf = (inf :: 'a multiset \<Rightarrow> _)"
-  ..
+lemma [code, code del]: "inf = (inf :: 'a multiset \<Rightarrow> _)" ..
 
-lemma [code, code del]:
-  "sup = (sup :: 'a multiset \<Rightarrow> _)"
-  ..
+lemma [code, code del]: "sup = (sup :: 'a multiset \<Rightarrow> _)" ..
 
-lemma [code, code del]:
-  "image_mset = image_mset"
-  ..
+lemma [code, code del]: "image_mset = image_mset" ..
 
-lemma [code, code del]:
-  "Multiset.filter = Multiset.filter"
-  ..
+lemma [code, code del]: "Multiset.filter = Multiset.filter" ..
 
-lemma [code, code del]:
-  "count = count"
-  ..
+lemma [code, code del]: "count = count" ..
 
-lemma [code, code del]:
-  "mcard = mcard"
-  ..
+lemma [code, code del]: "mcard = mcard" ..
 
-lemma [code, code del]:
-  "msetsum = msetsum"
-  ..
+lemma [code, code del]: "msetsum = msetsum" ..
 
-lemma [code, code del]:
-  "msetprod = msetprod"
-  ..
+lemma [code, code del]: "msetprod = msetprod" ..
 
-lemma [code, code del]:
-  "set_of = set_of"
-  ..
+lemma [code, code del]: "set_of = set_of" ..
 
-lemma [code, code del]:
-  "sorted_list_of_multiset = sorted_list_of_multiset"
-  ..
+lemma [code, code del]: "sorted_list_of_multiset = sorted_list_of_multiset" ..
 
-lemma [code, code del]:
-  "ord_multiset_inst.less_eq_multiset = ord_multiset_inst.less_eq_multiset"
-  ..
+lemma [code, code del]: "ord_multiset_inst.less_eq_multiset = ord_multiset_inst.less_eq_multiset" ..
 
-lemma [code, code del]:
-  "ord_multiset_inst.less_multiset = ord_multiset_inst.less_multiset"
-  ..
+lemma [code, code del]: "ord_multiset_inst.less_multiset = ord_multiset_inst.less_multiset" ..
 
-lemma [code, code del]:
-  "equal_multiset_inst.equal_multiset = equal_multiset_inst.equal_multiset"
-  ..
+lemma [code, code del]: "equal_multiset_inst.equal_multiset = equal_multiset_inst.equal_multiset" ..
 
 
-text {* Raw operations on lists *}
+text \<open>Raw operations on lists\<close>
 
-definition join_raw :: "('key \<Rightarrow> 'val \<times> 'val \<Rightarrow> 'val) \<Rightarrow> ('key \<times> 'val) list \<Rightarrow> ('key \<times> 'val) list \<Rightarrow> ('key \<times> 'val) list"
-where
-  "join_raw f xs ys = foldr (\<lambda>(k, v). map_default k v (%v'. f k (v', v))) ys xs"
+definition join_raw ::
+    "('key \<Rightarrow> 'val \<times> 'val \<Rightarrow> 'val) \<Rightarrow>
+      ('key \<times> 'val) list \<Rightarrow> ('key \<times> 'val) list \<Rightarrow> ('key \<times> 'val) list"
+  where "join_raw f xs ys = foldr (\<lambda>(k, v). map_default k v (\<lambda>v'. f k (v', v))) ys xs"
 
-lemma join_raw_Nil [simp]:
-  "join_raw f xs [] = xs"
-by (simp add: join_raw_def)
+lemma join_raw_Nil [simp]: "join_raw f xs [] = xs"
+  by (simp add: join_raw_def)
 
 lemma join_raw_Cons [simp]:
-  "join_raw f xs ((k, v) # ys) = map_default k v (%v'. f k (v', v)) (join_raw f xs ys)"
-by (simp add: join_raw_def)
+  "join_raw f xs ((k, v) # ys) = map_default k v (\<lambda>v'. f k (v', v)) (join_raw f xs ys)"
+  by (simp add: join_raw_def)
 
 lemma map_of_join_raw:
   assumes "distinct (map fst ys)"
-  shows "map_of (join_raw f xs ys) x = (case map_of xs x of None => map_of ys x | Some v =>
-    (case map_of ys x of None => Some v | Some v' => Some (f x (v, v'))))"
-using assms
-apply (induct ys)
-apply (auto simp add: map_of_map_default split: option.split)
-apply (metis map_of_eq_None_iff option.simps(2) weak_map_of_SomeI)
-by (metis Some_eq_map_of_iff map_of_eq_None_iff option.simps(2))
+  shows "map_of (join_raw f xs ys) x =
+    (case map_of xs x of
+      None \<Rightarrow> map_of ys x
+    | Some v \<Rightarrow> (case map_of ys x of None \<Rightarrow> Some v | Some v' \<Rightarrow> Some (f x (v, v'))))"
+  using assms
+  apply (induct ys)
+  apply (auto simp add: map_of_map_default split: option.split)
+  apply (metis map_of_eq_None_iff option.simps(2) weak_map_of_SomeI)
+  apply (metis Some_eq_map_of_iff map_of_eq_None_iff option.simps(2))
+  done
 
 lemma distinct_join_raw:
   assumes "distinct (map fst xs)"
   shows "distinct (map fst (join_raw f xs ys))"
-using assms
+  using assms
 proof (induct ys)
+  case Nil
+  then show ?case by simp
+next
   case (Cons y ys)
-  thus ?case by (cases y) (simp add: distinct_map_default)
-qed auto
+  then show ?case by (cases y) (simp add: distinct_map_default)
+qed
 
-definition
-  "subtract_entries_raw xs ys = foldr (%(k, v). AList.map_entry k (%v'. v' - v)) ys xs"
+definition "subtract_entries_raw xs ys = foldr (\<lambda>(k, v). AList.map_entry k (\<lambda>v'. v' - v)) ys xs"
 
 lemma map_of_subtract_entries_raw:
   assumes "distinct (map fst ys)"
-  shows "map_of (subtract_entries_raw xs ys) x = (case map_of xs x of None => None | Some v =>
-    (case map_of ys x of None => Some v | Some v' => Some (v - v')))"
-using assms unfolding subtract_entries_raw_def
-apply (induct ys)
-apply auto
-apply (simp split: option.split)
-apply (simp add: map_of_map_entry)
-apply (auto split: option.split)
-apply (metis map_of_eq_None_iff option.simps(3) option.simps(4))
-by (metis map_of_eq_None_iff option.simps(4) option.simps(5))
+  shows "map_of (subtract_entries_raw xs ys) x =
+    (case map_of xs x of
+      None \<Rightarrow> None
+    | Some v \<Rightarrow> (case map_of ys x of None \<Rightarrow> Some v | Some v' \<Rightarrow> Some (v - v')))"
+  using assms
+  unfolding subtract_entries_raw_def
+  apply (induct ys)
+  apply auto
+  apply (simp split: option.split)
+  apply (simp add: map_of_map_entry)
+  apply (auto split: option.split)
+  apply (metis map_of_eq_None_iff option.simps(3) option.simps(4))
+  apply (metis map_of_eq_None_iff option.simps(4) option.simps(5))
+  done
 
 lemma distinct_subtract_entries_raw:
   assumes "distinct (map fst xs)"
   shows "distinct (map fst (subtract_entries_raw xs ys))"
-using assms
-unfolding subtract_entries_raw_def by (induct ys) (auto simp add: distinct_map_entry)
+  using assms
+  unfolding subtract_entries_raw_def
+  by (induct ys) (auto simp add: distinct_map_entry)
 
 
-text {* Operations on alists with distinct keys *}
+text \<open>Operations on alists with distinct keys\<close>
 
-lift_definition join :: "('a \<Rightarrow> 'b \<times> 'b \<Rightarrow> 'b) \<Rightarrow> ('a, 'b) alist \<Rightarrow> ('a, 'b) alist \<Rightarrow> ('a, 'b) alist" 
-is join_raw
-by (simp add: distinct_join_raw)
+lift_definition join :: "('a \<Rightarrow> 'b \<times> 'b \<Rightarrow> 'b) \<Rightarrow> ('a, 'b) alist \<Rightarrow> ('a, 'b) alist \<Rightarrow> ('a, 'b) alist"
+  is join_raw
+  by (simp add: distinct_join_raw)
 
 lift_definition subtract_entries :: "('a, ('b :: minus)) alist \<Rightarrow> ('a, 'b) alist \<Rightarrow> ('a, 'b) alist"
-is subtract_entries_raw 
-by (simp add: distinct_subtract_entries_raw)
+  is subtract_entries_raw
+  by (simp add: distinct_subtract_entries_raw)
 
 
-text {* Implementing multisets by means of association lists *}
+text \<open>Implementing multisets by means of association lists\<close>
 
-definition count_of :: "('a \<times> nat) list \<Rightarrow> 'a \<Rightarrow> nat" where
-  "count_of xs x = (case map_of xs x of None \<Rightarrow> 0 | Some n \<Rightarrow> n)"
+definition count_of :: "('a \<times> nat) list \<Rightarrow> 'a \<Rightarrow> nat"
+  where "count_of xs x = (case map_of xs x of None \<Rightarrow> 0 | Some n \<Rightarrow> n)"
 
-lemma count_of_multiset:
-  "count_of xs \<in> multiset"
+lemma count_of_multiset: "count_of xs \<in> multiset"
 proof -
-  let ?A = "{x::'a. 0 < (case map_of xs x of None \<Rightarrow> 0\<Colon>nat | Some (n\<Colon>nat) \<Rightarrow> n)}"
+  let ?A = "{x::'a. 0 < (case map_of xs x of None \<Rightarrow> 0::nat | Some n \<Rightarrow> n)}"
   have "?A \<subseteq> dom (map_of xs)"
   proof
     fix x
     assume "x \<in> ?A"
-    then have "0 < (case map_of xs x of None \<Rightarrow> 0\<Colon>nat | Some (n\<Colon>nat) \<Rightarrow> n)" by simp
-    then have "map_of xs x \<noteq> None" by (cases "map_of xs x") auto
-    then show "x \<in> dom (map_of xs)" by auto
+    then have "0 < (case map_of xs x of None \<Rightarrow> 0::nat | Some n \<Rightarrow> n)"
+      by simp
+    then have "map_of xs x \<noteq> None"
+      by (cases "map_of xs x") auto
+    then show "x \<in> dom (map_of xs)"
+      by auto
   qed
   with finite_dom_map_of [of xs] have "finite ?A"
     by (auto intro: finite_subset)
@@ -174,82 +152,80 @@ lemma count_simps [simp]:
   "count_of ((x, n) # xs) = (\<lambda>y. if x = y then n else count_of xs y)"
   by (simp_all add: count_of_def fun_eq_iff)
 
-lemma count_of_empty:
-  "x \<notin> fst ` set xs \<Longrightarrow> count_of xs x = 0"
+lemma count_of_empty: "x \<notin> fst ` set xs \<Longrightarrow> count_of xs x = 0"
   by (induct xs) (simp_all add: count_of_def)
 
-lemma count_of_filter:
-  "count_of (List.filter (P \<circ> fst) xs) x = (if P x then count_of xs x else 0)"
+lemma count_of_filter: "count_of (List.filter (P \<circ> fst) xs) x = (if P x then count_of xs x else 0)"
   by (induct xs) auto
 
 lemma count_of_map_default [simp]:
-  "count_of (map_default x b (%x. x + b) xs) y = (if x = y then count_of xs x + b else count_of xs y)"
-unfolding count_of_def by (simp add: map_of_map_default split: option.split)
+  "count_of (map_default x b (\<lambda>x. x + b) xs) y =
+    (if x = y then count_of xs x + b else count_of xs y)"
+  unfolding count_of_def by (simp add: map_of_map_default split: option.split)
 
 lemma count_of_join_raw:
-  "distinct (map fst ys) ==> count_of xs x + count_of ys x = count_of (join_raw (%x (x, y). x + y) xs ys) x"
-unfolding count_of_def by (simp add: map_of_join_raw split: option.split)
+  "distinct (map fst ys) \<Longrightarrow>
+    count_of xs x + count_of ys x = count_of (join_raw (\<lambda>x (x, y). x + y) xs ys) x"
+  unfolding count_of_def by (simp add: map_of_join_raw split: option.split)
 
 lemma count_of_subtract_entries_raw:
-  "distinct (map fst ys) ==> count_of xs x - count_of ys x = count_of (subtract_entries_raw xs ys) x"
-unfolding count_of_def by (simp add: map_of_subtract_entries_raw split: option.split)
+  "distinct (map fst ys) \<Longrightarrow>
+    count_of xs x - count_of ys x = count_of (subtract_entries_raw xs ys) x"
+  unfolding count_of_def by (simp add: map_of_subtract_entries_raw split: option.split)
 
 
-text {* Code equations for multiset operations *}
+text \<open>Code equations for multiset operations\<close>
 
-definition Bag :: "('a, nat) alist \<Rightarrow> 'a multiset" where
-  "Bag xs = Abs_multiset (count_of (DAList.impl_of xs))"
+definition Bag :: "('a, nat) alist \<Rightarrow> 'a multiset"
+  where "Bag xs = Abs_multiset (count_of (DAList.impl_of xs))"
 
 code_datatype Bag
 
-lemma count_Bag [simp, code]:
-  "count (Bag xs) = count_of (DAList.impl_of xs)"
-  by (simp add: Bag_def count_of_multiset Abs_multiset_inverse)
+lemma count_Bag [simp, code]: "count (Bag xs) = count_of (DAList.impl_of xs)"
+  by (simp add: Bag_def count_of_multiset)
 
-lemma Mempty_Bag [code]:
-  "{#} = Bag (DAList.empty)"
+lemma Mempty_Bag [code]: "{#} = Bag (DAList.empty)"
   by (simp add: multiset_eq_iff alist.Alist_inverse DAList.empty_def)
 
-lemma single_Bag [code]:
-  "{#x#} = Bag (DAList.update x 1 DAList.empty)"
+lemma single_Bag [code]: "{#x#} = Bag (DAList.update x 1 DAList.empty)"
   by (simp add: multiset_eq_iff alist.Alist_inverse update.rep_eq empty.rep_eq)
 
-lemma union_Bag [code]:
-  "Bag xs + Bag ys = Bag (join (\<lambda>x (n1, n2). n1 + n2) xs ys)"
-by (rule multiset_eqI) (simp add: count_of_join_raw alist.Alist_inverse distinct_join_raw join_def)
+lemma union_Bag [code]: "Bag xs + Bag ys = Bag (join (\<lambda>x (n1, n2). n1 + n2) xs ys)"
+  by (rule multiset_eqI)
+    (simp add: count_of_join_raw alist.Alist_inverse distinct_join_raw join_def)
 
-lemma minus_Bag [code]:
-  "Bag xs - Bag ys = Bag (subtract_entries xs ys)"
-by (rule multiset_eqI)
-  (simp add: count_of_subtract_entries_raw alist.Alist_inverse distinct_subtract_entries_raw subtract_entries_def)
+lemma minus_Bag [code]: "Bag xs - Bag ys = Bag (subtract_entries xs ys)"
+  by (rule multiset_eqI)
+    (simp add: count_of_subtract_entries_raw alist.Alist_inverse
+      distinct_subtract_entries_raw subtract_entries_def)
 
-lemma filter_Bag [code]:
-  "Multiset.filter P (Bag xs) = Bag (DAList.filter (P \<circ> fst) xs)"
-by (rule multiset_eqI) (simp add: count_of_filter DAList.filter.rep_eq)
+lemma filter_Bag [code]: "Multiset.filter P (Bag xs) = Bag (DAList.filter (P \<circ> fst) xs)"
+  by (rule multiset_eqI) (simp add: count_of_filter DAList.filter.rep_eq)
 
 
 lemma mset_eq [code]: "HOL.equal (m1::'a::equal multiset) m2 \<longleftrightarrow> m1 \<le> m2 \<and> m2 \<le> m1"
-by (metis equal_multiset_def eq_iff)
+  by (metis equal_multiset_def eq_iff)
 
-text{* By default the code for @{text "<"} is @{prop"xs < ys \<longleftrightarrow> xs \<le> ys \<and> \<not> xs = ys"}.
+text \<open>By default the code for @{text "<"} is @{prop"xs < ys \<longleftrightarrow> xs \<le> ys \<and> \<not> xs = ys"}.
 With equality implemented by @{text"\<le>"}, this leads to three calls of  @{text"\<le>"}.
-Here is a more efficient version: *}
-lemma mset_less[code]: "xs < (ys :: 'a multiset) \<longleftrightarrow> xs \<le> ys \<and> \<not> ys \<le> xs" 
-by (rule less_le_not_le)
+Here is a more efficient version:\<close>
+lemma mset_less[code]: "xs < (ys :: 'a multiset) \<longleftrightarrow> xs \<le> ys \<and> \<not> ys \<le> xs"
+  by (rule less_le_not_le)
 
 lemma mset_less_eq_Bag0:
   "Bag xs \<le> A \<longleftrightarrow> (\<forall>(x, n) \<in> set (DAList.impl_of xs). count_of (DAList.impl_of xs) x \<le> count A x)"
     (is "?lhs \<longleftrightarrow> ?rhs")
 proof
-  assume ?lhs thus ?rhs by (auto simp add: mset_le_def)
+  assume ?lhs
+  then show ?rhs by (auto simp add: mset_le_def)
 next
   assume ?rhs
   show ?lhs
   proof (rule mset_less_eqI)
     fix x
-    from `?rhs` have "count_of (DAList.impl_of xs) x \<le> count A x"
+    from \<open>?rhs\<close> have "count_of (DAList.impl_of xs) x \<le> count A x"
       by (cases "x \<in> fst ` set (DAList.impl_of xs)") (auto simp add: count_of_empty)
-    thus "count (Bag xs) x \<le> count A x" by (simp add: mset_le_def)
+    then show "count (Bag xs) x \<le> count A x" by (simp add: mset_le_def)
   qed
 qed
 
@@ -259,27 +235,34 @@ proof -
   {
     fix x n
     assume "(x,n) \<in> set (DAList.impl_of xs)"
-    hence "count_of (DAList.impl_of xs) x = n" 
-    proof (transfer)
-      fix x n and xs :: "('a \<times> nat) list"
+    then have "count_of (DAList.impl_of xs) x = n"
+    proof transfer
+      fix x n
+      fix xs :: "('a \<times> nat) list"
       show "(distinct \<circ> map fst) xs \<Longrightarrow> (x, n) \<in> set xs \<Longrightarrow> count_of xs x = n"
-      proof (induct xs) 
-        case (Cons ym ys)        
+      proof (induct xs)
+        case Nil
+        then show ?case by simp
+      next
+        case (Cons ym ys)
         obtain y m where ym: "ym = (y,m)" by force
         note Cons = Cons[unfolded ym]
         show ?case
         proof (cases "x = y")
           case False
-          with Cons show ?thesis unfolding ym by auto
+          with Cons show ?thesis
+            unfolding ym by auto
         next
           case True
           with Cons(2-3) have "m = n" by force
-          with True show ?thesis unfolding ym by auto
+          with True show ?thesis
+            unfolding ym by auto
         qed
-      qed auto
+      qed
     qed
   }
-  thus ?thesis unfolding mset_less_eq_Bag0 by auto
+  then show ?thesis
+    unfolding mset_less_eq_Bag0 by auto
 qed
 
 declare multiset_inter_def [code]
@@ -287,29 +270,31 @@ declare sup_multiset_def [code]
 declare multiset_of.simps [code]
 
 
-fun fold_impl :: "('a \<Rightarrow> nat \<Rightarrow> 'b \<Rightarrow> 'b) \<Rightarrow> 'b \<Rightarrow> ('a \<times> nat)list \<Rightarrow> 'b" where
+fun fold_impl :: "('a \<Rightarrow> nat \<Rightarrow> 'b \<Rightarrow> 'b) \<Rightarrow> 'b \<Rightarrow> ('a \<times> nat) list \<Rightarrow> 'b"
+where
   "fold_impl fn e ((a,n) # ms) = (fold_impl fn ((fn a n) e) ms)"
 | "fold_impl fn e [] = e"
 
-definition fold :: "('a \<Rightarrow> nat \<Rightarrow> 'b \<Rightarrow> 'b) \<Rightarrow> 'b \<Rightarrow> ('a, nat)alist \<Rightarrow> 'b" where
-"fold f e al = fold_impl f e (DAList.impl_of al)"
+definition fold :: "('a \<Rightarrow> nat \<Rightarrow> 'b \<Rightarrow> 'b) \<Rightarrow> 'b \<Rightarrow> ('a, nat) alist \<Rightarrow> 'b"
+  where "fold f e al = fold_impl f e (DAList.impl_of al)"
 
 hide_const (open) fold
 
 context comp_fun_commute
 begin
 
-lemma DAList_Multiset_fold: assumes fn: "\<And> a n x. fn a n x = (f a ^^ n) x"
+lemma DAList_Multiset_fold:
+  assumes fn: "\<And>a n x. fn a n x = (f a ^^ n) x"
   shows "Multiset.fold f e (Bag al) = DAList_Multiset.fold fn e al"
-unfolding DAList_Multiset.fold_def
+  unfolding DAList_Multiset.fold_def
 proof (induct al)
   fix ys
-  let ?inv = "{xs :: ('a \<times> nat)list. (distinct \<circ> map fst) xs}"
+  let ?inv = "{xs :: ('a \<times> nat) list. (distinct \<circ> map fst) xs}"
   note cs[simp del] = count_simps
-  have count[simp]: "\<And> x. count (Abs_multiset (count_of x)) = count_of x"
+  have count[simp]: "\<And>x. count (Abs_multiset (count_of x)) = count_of x"
     by (rule Abs_multiset_inverse[OF count_of_multiset])
   assume ys: "ys \<in> ?inv"
-  thus "Multiset.fold f e (Bag (Alist ys)) = fold_impl fn e (DAList.impl_of (Alist ys))"
+  then show "Multiset.fold f e (Bag (Alist ys)) = fold_impl fn e (DAList.impl_of (Alist ys))"
     unfolding Bag_def unfolding Alist_inverse[OF ys]
   proof (induct ys arbitrary: e rule: list.induct)
     case Nil
@@ -318,114 +303,136 @@ proof (induct al)
          (auto, simp add: cs)
   next
     case (Cons pair ys e)
-    obtain a n where pair: "pair = (a,n)" by force
-    from fn[of a n] have [simp]: "fn a n = (f a ^^ n)" by auto
-    have inv: "ys \<in> ?inv" using Cons(2) by auto
+    obtain a n where pair: "pair = (a,n)"
+      by force
+    from fn[of a n] have [simp]: "fn a n = (f a ^^ n)"
+      by auto
+    have inv: "ys \<in> ?inv"
+      using Cons(2) by auto
     note IH = Cons(1)[OF inv]
     def Ys \<equiv> "Abs_multiset (count_of ys)"
     have id: "Abs_multiset (count_of ((a, n) # ys)) = ((op + {# a #}) ^^ n) Ys"
       unfolding Ys_def
     proof (rule multiset_eqI, unfold count)
-      fix c      
-      show "count_of ((a, n) # ys) c = count ((op + {#a#} ^^ n) (Abs_multiset (count_of ys))) c" (is "?l = ?r")
+      fix c
+      show "count_of ((a, n) # ys) c =
+        count ((op + {#a#} ^^ n) (Abs_multiset (count_of ys))) c" (is "?l = ?r")
       proof (cases "c = a")
-        case False thus ?thesis unfolding cs by (induct n) auto
+        case False
+        then show ?thesis
+          unfolding cs by (induct n) auto
       next
         case True
-        hence "?l = n" by (simp add: cs)
+        then have "?l = n" by (simp add: cs)
         also have "n = ?r" unfolding True
         proof (induct n)
           case 0
           from Cons(2)[unfolded pair] have "a \<notin> fst ` set ys" by auto
-          thus ?case by (induct ys) (simp, auto simp: cs)
-        qed auto
+          then show ?case by (induct ys) (simp, auto simp: cs)
+        next
+          case Suc
+          then show ?case by simp
+        qed
         finally show ?thesis .
       qed
     qed
-    show ?case unfolding pair    
-      by (simp add: IH[symmetric], unfold id Ys_def[symmetric],
-      induct n, auto simp: fold_mset_fun_left_comm[symmetric])
+    show ?case
+      unfolding pair
+      apply (simp add: IH[symmetric])
+      unfolding id Ys_def[symmetric]
+      apply (induct n)
+      apply (auto simp: fold_mset_fun_left_comm[symmetric])
+      done
   qed
 qed
 
-end 
+end
 
-lift_definition single_alist_entry :: "'a \<Rightarrow> 'b \<Rightarrow> ('a,'b)alist" is "\<lambda> a b. [(a,b)]" by auto
+lift_definition single_alist_entry :: "'a \<Rightarrow> 'b \<Rightarrow> ('a, 'b) alist" is "\<lambda>a b. [(a, b)]"
+  by auto
 
-lemma image_mset_Bag[code]:
+lemma image_mset_Bag [code]:
   "image_mset f (Bag ms) =
-   DAList_Multiset.fold (\<lambda> a n m. Bag (single_alist_entry (f a) n) + m) {#} ms"
-unfolding image_mset_def 
+    DAList_Multiset.fold (\<lambda>a n m. Bag (single_alist_entry (f a) n) + m) {#} ms"
+  unfolding image_mset_def
 proof (rule comp_fun_commute.DAList_Multiset_fold, unfold_locales, (auto simp: ac_simps)[1])
   fix a n m
   show "Bag (single_alist_entry (f a) n) + m = ((op + \<circ> single \<circ> f) a ^^ n) m" (is "?l = ?r")
   proof (rule multiset_eqI)
     fix x
     have "count ?r x = (if x = f a then n + count m x else count m x)"
-      by (induct n, auto)
-    also have "\<dots> = count ?l x" by (simp add: single_alist_entry.rep_eq)
+      by (induct n) auto
+    also have "\<dots> = count ?l x"
+      by (simp add: single_alist_entry.rep_eq)
     finally show "count ?l x = count ?r x" ..
   qed
 qed
 
 hide_const single_alist_entry
 
-(* we cannot use (\<lambda> a n. op + (a * n)) for folding, since * is not defined
+(* we cannot use (\<lambda>a n. op + (a * n)) for folding, since * is not defined
    in comm_monoid_add *)
-lemma msetsum_Bag[code]:
-  "msetsum (Bag ms) = DAList_Multiset.fold (\<lambda> a n. ((op + a) ^^ n)) 0 ms"
-unfolding msetsum.eq_fold
-by (rule comp_fun_commute.DAList_Multiset_fold, unfold_locales, auto simp: ac_simps)
+lemma msetsum_Bag[code]: "msetsum (Bag ms) = DAList_Multiset.fold (\<lambda>a n. ((op + a) ^^ n)) 0 ms"
+  unfolding msetsum.eq_fold
+  apply (rule comp_fun_commute.DAList_Multiset_fold)
+  apply unfold_locales
+  apply (auto simp: ac_simps)
+  done
 
-(* we cannot use (\<lambda> a n. op * (a ^ n)) for folding, since ^ is not defined
+(* we cannot use (\<lambda>a n. op * (a ^ n)) for folding, since ^ is not defined
    in comm_monoid_mult *)
-lemma msetprod_Bag[code]:
-  "msetprod (Bag ms) = DAList_Multiset.fold (\<lambda> a n. ((op * a) ^^ n)) 1 ms"
-unfolding msetprod.eq_fold
-by (rule comp_fun_commute.DAList_Multiset_fold, unfold_locales, auto simp: ac_simps)
+lemma msetprod_Bag[code]: "msetprod (Bag ms) = DAList_Multiset.fold (\<lambda>a n. ((op * a) ^^ n)) 1 ms"
+  unfolding msetprod.eq_fold
+  apply (rule comp_fun_commute.DAList_Multiset_fold)
+  apply unfold_locales
+  apply (auto simp: ac_simps)
+  done
 
-lemma mcard_fold: "mcard A = Multiset.fold (\<lambda> _. Suc) 0 A" (is "_ = Multiset.fold ?f _ _")
+lemma mcard_fold: "mcard A = Multiset.fold (\<lambda>_. Suc) 0 A" (is "_ = Multiset.fold ?f _ _")
 proof -
-  interpret comp_fun_commute ?f by (default, auto)
+  interpret comp_fun_commute ?f by default auto
   show ?thesis by (induct A) auto
 qed
 
-lemma mcard_Bag[code]:
-  "mcard (Bag ms) = DAList_Multiset.fold (\<lambda> a n. op + n) 0 ms"
-unfolding mcard_fold
+lemma mcard_Bag[code]: "mcard (Bag ms) = DAList_Multiset.fold (\<lambda>a n. op + n) 0 ms"
+  unfolding mcard_fold
 proof (rule comp_fun_commute.DAList_Multiset_fold, unfold_locales, simp)
   fix a n x
-  show "n + x = (Suc ^^ n) x" by (induct n) auto
+  show "n + x = (Suc ^^ n) x"
+    by (induct n) auto
 qed
 
 
 lemma set_of_fold: "set_of A = Multiset.fold insert {} A" (is "_ = Multiset.fold ?f _ _")
 proof -
-  interpret comp_fun_commute ?f by (default, auto)
-  show ?thesis by (induct A, auto)
+  interpret comp_fun_commute ?f by default auto
+  show ?thesis by (induct A) auto
 qed
 
 lemma set_of_Bag[code]:
-  "set_of (Bag ms) = DAList_Multiset.fold (\<lambda> a n. (if n = 0 then (\<lambda> m. m) else insert a)) {} ms"
-unfolding set_of_fold
+  "set_of (Bag ms) = DAList_Multiset.fold (\<lambda>a n. (if n = 0 then (\<lambda>m. m) else insert a)) {} ms"
+  unfolding set_of_fold
 proof (rule comp_fun_commute.DAList_Multiset_fold, unfold_locales, (auto simp: ac_simps)[1])
   fix a n x
   show "(if n = 0 then \<lambda>m. m else insert a) x = (insert a ^^ n) x" (is "?l n = ?r n")
   proof (cases n)
+    case 0
+    then show ?thesis by simp
+  next
     case (Suc m)
-    hence "?l n = insert a x" by simp
+    then have "?l n = insert a x" by simp
     moreover have "?r n = insert a x" unfolding Suc by (induct m) auto
     ultimately show ?thesis by auto
-  qed auto
+  qed
 qed
 
 
 instantiation multiset :: (exhaustive) exhaustive
 begin
 
-definition exhaustive_multiset :: "('a multiset \<Rightarrow> (bool \<times> term list) option) \<Rightarrow> natural \<Rightarrow> (bool * term list) option"
-where
-  "exhaustive_multiset f i = Quickcheck_Exhaustive.exhaustive (\<lambda>xs. f (Bag xs)) i"
+definition exhaustive_multiset ::
+  "('a multiset \<Rightarrow> (bool \<times> term list) option) \<Rightarrow> natural \<Rightarrow> (bool \<times> term list) option"
+  where "exhaustive_multiset f i = Quickcheck_Exhaustive.exhaustive (\<lambda>xs. f (Bag xs)) i"
 
 instance ..
 
